{
 "cells": [
  {
   "cell_type": "markdown",
   "id": "a4e0f691",
   "metadata": {},
   "source": [
    "(week4)=\n",
    "\n",
    "# Week4 -  fundamental equation of mechanics\n",
    "\n",
    "\\begin{eqnarray*}\n",
    "&mx''& = &-kx& - &cx'&\\\\\n",
    "&\\uparrow& &\\uparrow& &\\uparrow&\\\\\n",
    "&\\text{Force (Newton)}& &\\text{spring (Hooke)}& &\\text{dash pot/damping}&\n",
    "\\end{eqnarray*}\n",
    "\n",
    "\\begin{eqnarray*}\n",
    "\\Longrightarrow mx''+cx'+kx=0\\\\\\\\\n",
    "\\Longrightarrow x''+ \\frac{c}{m}x'+ \\frac{k}{m}x=0\n",
    "\\end{eqnarray*}\n",
    "\n",
    "```{figure} /_static/figures/car_ode.jpeg\n",
    ":scale: 10%\n",
    ":name: car\n",
    "```\n",
    "\n",
    "## Second order linear (homogeneous) ODEs\n",
    "- to find two independent solutions (homogeneous solutions)\n",
    "- general form: \n",
    "\\begin{eqnarray*}\n",
    "\\frac{d^{2}y}{dt^{2}}+A\\frac{dy}{dt}+By=0, \\text{ given } y(0)=1, y'(0)=0.\n",
    "\\end{eqnarray*}\n",
    "- basic method guess and plug in the exponential solution:\n",
    "\\begin{eqnarray*}\n",
    "\\text{try } y(t)&=&e^{rt}\\\\\\\\ \n",
    "\\rightarrow r^{2}e^{rt} + Are^{rt} &+& Be^{rt} = 0\\\\\\\\\n",
    "\\rightarrow r^{2} + Ar &+& B = 0 \\text{ characteristic equation}.\n",
    "\\end{eqnarray*}\n",
    "\n",
    "- we can solve r:\n",
    "\\begin{eqnarray*}\n",
    "r=\\frac{-A\\pm \\sqrt{A^{2}-4B}}{2}\n",
    "\\end{eqnarray*}\n",
    "\n",
    "## Case1: two real roots (overdamping)\n",
    "\\begin{eqnarray*}\n",
    "r_{1} \\neq r_{2} \\rightarrow y(t)=c_{1}e^{r_{1}t}+c_{2}e^{r_{2}t}\n",
    "\\end{eqnarray*}\n",
    "\n",
    "````{prf:example}\n",
    ":label: my-example1\n",
    "\n",
    "\\begin{eqnarray*}\n",
    "y''+4y'+3y=0, y(0)=1, y'(0)=0\n",
    "\\end{eqnarray*}\n",
    "\n",
    "The characteristic equation is\n",
    "\\begin{eqnarray*}\n",
    "r^{2}&+&4r+3=0\\\\\\\\\n",
    "&\\Longrightarrow& (r+3)(r+1)=0 \\rightarrow r=-3, -1\\\\\\\\\n",
    "&\\Longrightarrow& y(t)=c_{1}e^{-3t}+c_{2}e^{-t}\n",
    "\\end{eqnarray*}\n",
    "\n",
    "Use initial conditions\n",
    "\\begin{eqnarray*}\n",
    "y(0)&=&1=c_{1}+c_{2}, \\\\\\\\\n",
    "y'(0)&=&0=-3c_{1}-c_{2}\\\\\\\\\n",
    "&\\Longrightarrow& c_{1}=\\frac{-1}{2}, c_{2}=\\frac{3}{2}\\\\\\\\\n",
    "&\\Longrightarrow& y(t)=\\frac{-1}{2}e^{-3t}+\\frac{3}{2}e^{-t}\n",
    "\\end{eqnarray*}\n",
    "````\n",
    "\n",
    "```{note}\n",
    "Why the solutions are always \"damped\"? Can you link this result to the value of r?\n",
    "```\n",
    "\n",
    "- the plot for possible solutions y(t):\n",
    "```{figure} /_static/figures/overdamp.png\n",
    ":scale: 50%\n",
    ":name: overdamp\n",
    "```\n",
    "\n",
    "## Case2: two equal roots (critical damping)\n",
    "\\begin{eqnarray*}\n",
    "r_{1} = r_{2} = -a \\rightarrow (r+a)^{2}=0 \\rightarrow r^{2}+2ar+a^{2}=0.\n",
    "\\end{eqnarray*}\n",
    "\n",
    "So the ODE can be expressed as:\n",
    "\\begin{eqnarray*}\n",
    "y''+2ay'+a^{2}y=0.\n",
    "\\end{eqnarray*}\n",
    "\n",
    "Now we only have one solution:\n",
    "\\begin{eqnarray*}\n",
    "y(t)=e^{-at}=y_{1}(t)\n",
    "\\end{eqnarray*}\n",
    "\n",
    "But we need one more. Let's try this:\n",
    "\\begin{eqnarray*}\n",
    "\\text{let } y_{2}(t)=u(t)y_{1}(t)\\\\\\\\\n",
    "a^{2}&\\times& (y_{2} = ue^{-at})\\\\\\\\\n",
    "2a&\\times& (y_{2}'=u(-ae^{-at}) +u'e^{-at})\\\\\\\\\n",
    "1&\\times& (y_{2}''=a^{2}e^{-at}u-ae^{-at}u'-ae^{-at}u'+e^{-at}u'')\\\\\\\\\n",
    "&\\Longrightarrow& 0 = 0 + 0 + e^{-at}u''\\\\\\\\\n",
    "&\\Longrightarrow& u'' = 0 \\rightarrow u'=c_{1} \\rightarrow u(t) = c_{1}t+c_{2}.\n",
    "\\end{eqnarray*}\n",
    "\n",
    "We take another solution and obtain the general solution:\n",
    "\\begin{eqnarray*}\n",
    "y_{2}(t) &=& te^{-at}\\\\\\\\\n",
    "y(t) &=& Cy_{1}(t) + Dy_{2}(t) = Ce^{-at}+Dte^{-at}\n",
    "\\end{eqnarray*}\n",
    "\n",
    "## Case 3: complex roots (undamped/underdamped)\n",
    "We get the complex solution\n",
    "\\begin{eqnarray*}\n",
    "y_{c}(t) = e^{(a+bi)t} = u + iv, \\text{ where } u, v \\in \\mathbb{R}\n",
    "\\end{eqnarray*}\n",
    "\n",
    "````{prf:theorem}\n",
    ":label: my-theorem\n",
    "\n",
    "If u+iv is the complex solution to\n",
    "\n",
    "\\begin{eqnarray*}\n",
    "y''+Ay'+By = 0,\n",
    "\\end{eqnarray*}\n",
    "\n",
    "where A and B are real. Then u and v are real solutions.\n",
    "\n",
    "````\n",
    "\n",
    "````{prf:proof}\n",
    ":class: dropdown\n",
    "Plug the complex solution into the ODE:\n",
    "\n",
    "\\begin{eqnarray*}\n",
    "(u+iv)'' + A(u+iv)' + B(u+iv) = 0\\\\\\\\\n",
    "\\Longrightarrow (u''+Au'+Bu) + i(v''+Av'+Bv) = 0.\n",
    "\\end{eqnarray*}\n",
    "\n",
    "The only way that this equation holds is the real part equal to zero and imaginary part equal to zero. \n",
    "So the linear combination of u and v is the general solution:\n",
    "\n",
    "\\begin{eqnarray*}\n",
    "y(t) = c_{1}u(t) + c_{2}v(t)\n",
    "\\end{eqnarray*}\n",
    "\n",
    "````\n",
    "So the complex solution is\n",
    "\\begin{eqnarray*}\n",
    "\\tilde{y_c}(t) = e^{at+ibt}=e^{at}\\cos{bt} + ie^{at}\\sin{bt}.\n",
    "\\end{eqnarray*}\n",
    "\n",
    "And the general solution is\n",
    "\\begin{eqnarray*}\n",
    "y(t) = e^{at}(c_{1}\\cos{bt} + c_{2}\\sin{bt})\n",
    "\\end{eqnarray*}\n",
    "\n",
    "```{note}\n",
    "How about considering this complex solution\n",
    "\\begin{eqnarray*}\n",
    "y_{c}(t) = e^{at-ibt} \\text{?}\n",
    "\\end{eqnarray*}\n",
    "Can we obtain the same general solution? And why?\n",
    "```\n",
    "\n",
    "````{prf:example}\n",
    ":label: my-example2\n",
    "\n",
    "\\begin{eqnarray*}\n",
    "y''+4y'+5y=0, y(0)=1, y'(0)=0\n",
    "\\end{eqnarray*}\n",
    "\n",
    "The characteristic equation is\n",
    "\\begin{eqnarray*}\n",
    "r^{2}&+&4r+5=0\\\\\\\\\n",
    "&\\Longrightarrow& r=\\frac{-4\\pm \\sqrt{-4}}{2} = -2\\pm i\\\\\\\\\n",
    "\\end{eqnarray*}\n",
    "\n",
    "So the complex solution is:\n",
    "\\begin{eqnarray*}\n",
    "e^{(-2\\pm i)t} \\rightarrow e^{-2t}(\\cos{t}\\pm \\sin{t})\n",
    "\\end{eqnarray*}\n",
    "\n",
    "The general solution is therefore:\n",
    "\\begin{eqnarray*}\n",
    "y(t) &=& e^{-2t}(c_{1}\\cos{t}+c_{2}\\sin{t})\\\\\\\\\n",
    "y'(t) &=& -2e^{-2t}(c_{1}\\cos{t}+c_{2}\\sin{t}) + e^{-2t}(-c_{1}\\sin{t}+c_{2}\\cos{t})\n",
    "\\end{eqnarray*}\n",
    "\n",
    "Use initial conditions\n",
    "\\begin{eqnarray*}\n",
    "y(0)&=&1=c_{1}, \\\\\\\\\n",
    "y'(0)&=&0=-2c_{1}+c_{2} \\rightarrow c_{2}=2\\\\\\\\\n",
    "&\\Longrightarrow& y(t)=e^{-2t}(\\cos{t}+2\\sin{t})=\\sqrt{5}e^{-2t}\\cos{}(t-\\phi)\n",
    "\\end{eqnarray*}\n",
    "\n",
    "This is a solution underdamped.\n",
    "\n",
    "````\n",
    "\n",
    "Let us now revisit the problem with slightly modification on the coefficients:\n",
    "\\begin{eqnarray*}\n",
    "y'' &+& 2py'+\\omega_{o}^{2}y=0,\\\\\\\\\n",
    "\\text{where } &\\omega_{o}& \\text{is the natural frequency and p represents the damping.} \n",
    "\\end{eqnarray*}\n",
    "\n",
    "The characteristic equation is\n",
    "\\begin{eqnarray*}\n",
    "r^{2} + 2pr + \\omega_{o}^{2} = 0 \\\\\\\\\n",
    "\\rightarrow r = -p \\pm \\sqrt{p^{2}-\\omega_{o}^{2}}\n",
    "\\end{eqnarray*}\n",
    "\n",
    "- if p=0, then there is no damping or called undamped.\n",
    "\\begin{eqnarray*}\n",
    "&&y''+\\omega_{o}^{2}y=0\\\\\\\\\n",
    "&\\Longrightarrow& r=\\pm i\\omega_{o}\\\\\\\\\n",
    "&\\Longrightarrow& y(t) = c_{1}\\cos{\\omega_{o}t} + c_{2}\\sin{\\omega_{o}t} = A\\cos{}(\\omega_{o}t-\\phi)\n",
    "\\end{eqnarray*}\n",
    "\n",
    "- if another case\n",
    "\\begin{eqnarray*}\n",
    "p^{2}-\\omega_{o}^{2} < 0 \\rightarrow p<\\omega_{o},\n",
    "\\end{eqnarray*}\n",
    "then we call the solution underdamped.\n",
    "\n",
    "````{prf:definition}\n",
    ":label: my-definition1\n",
    "We define the pseudo-frequency as:\n",
    "\\begin{eqnarray*}\n",
    "\\omega_{d}^{2} = \\omega_{o}^{2} - p^{2}\n",
    "\\end{eqnarray*}\n",
    "````\n",
    "\n",
    "\\begin{eqnarray*}\n",
    "r = -p \\pm \\sqrt{-\\omega_{d}^{2}} = -p \\pm i\\omega_{d}\n",
    "\\end{eqnarray*}\n",
    "\n",
    "So the general solution is\n",
    "\\begin{eqnarray*}\n",
    "y(t) &=& e^{-pt}(c_{1}\\cos{}(\\omega_{d}t) + c_{2}\\sin{}(\\omega_{d})) \\\\\\\\\n",
    "&=& Ae^{-pt}\\cos{}(\\omega_{d}t-\\phi)\n",
    "\\end{eqnarray*}\n",
    "\n",
    "## Similarity between electrical and spring-dash pot system\n",
    "```{figure} /_static/figures/similarity_ode.jpeg\n",
    ":scale: 20%\n",
    ":name: similar\n",
    "```"
   ]
  }
 ],
 "metadata": {
  "jupytext": {
   "text_representation": {
    "extension": ".md",
    "format_name": "myst"
   }
  },
  "kernelspec": {
   "display_name": "Python 3",
   "language": "python",
   "name": "python3"
  },
  "source_map": [
   10
  ]
 },
 "nbformat": 4,
 "nbformat_minor": 5
}