{
 "cells": [
  {
   "cell_type": "markdown",
   "id": "582efb81",
   "metadata": {},
   "source": [
    "(week6)=\n",
    "\n",
    "# Week6 - exponential response formula (ERF)\n",
    "This method gives us guide to find the nonhomogeneous (particular) solutions for exponential-type forcing or source term.\n",
    "Consider the second order ODE:\n",
    "\\begin{eqnarray*}\n",
    "A''+by'+cy &=& e^{\\alpha x}, \\alpha \\in \\mathbb{C} \\\\\\\\\n",
    "&=& e^{(a+i\\omega)x}\\\\\\\\\n",
    "\\Longrightarrow (D^{2}+AD+B)y &=& P(D)y = e^{\\alpha x}\n",
    "\\end{eqnarray*}\n",
    "\n",
    "Below exponential inputs are all special cases of exponential function\n",
    "\\begin{eqnarray*}\n",
    "e^{ax}, \\sin{}(\\omega x), \\cos{}(\\omega x), e^{ax}\\sin{}(\\omega x), e^{ax}\\cos{}(\\omega x)\n",
    "\\end{eqnarray*}\n",
    "\n",
    "\n",
    "````{prf:example}\n",
    ":label: my-example_erf1\n",
    "\\begin{eqnarray*}\n",
    "P(D)e^{\\alpha x} = P(\\alpha)e^{\\alpha x}\n",
    "\\end{eqnarray*}\n",
    "````\n",
    "\n",
    "````{prf:theorem}\n",
    ":label: my-theorem_erf1\n",
    "Exponential-input theorem\n",
    "\n",
    "\\begin{eqnarray*}\n",
    "y_{p} = \\frac{e^{\\alpha x}}{p(\\alpha)} \\text{ solves } P(D)y=e^{\\alpha x}\n",
    "\\end{eqnarray*}\n",
    "````\n",
    "\n",
    "````{prf:proof}\n",
    "if \n",
    "\\begin{eqnarray*}\n",
    "P(D)y_{p} = e^{\\alpha x},\n",
    "\\end{eqnarray*}\n",
    "then\n",
    "\\begin{eqnarray*}\n",
    "P(D)\\frac{e^{\\alpha x}}{P(\\alpha)} = \\frac{1}{P(\\alpha)}P(D)e^{\\alpha x} = \\frac{1}{P(\\alpha)}P(\\alpha)e^{\\alpha x} = e^{\\alpha x}\n",
    "\\end{eqnarray*}\n",
    "\n",
    "````\n",
    "\n",
    "````{prf:example}\n",
    ":label: my-example_erf2\n",
    "\\begin{eqnarray*}\n",
    "y''-y'+2y=10e^{-x}\\sin{}(x)\n",
    "\\end{eqnarray*}\n",
    "\n",
    "We first complixy the ODE, solve the particular solution, and find its imaginary part:\n",
    "\\begin{eqnarray*}\n",
    "\\tilde{y_{p}}'' - \\tilde{y_{p}}' + 2\\tilde{y_{p}} &=& 10e^{(-1+i)x} \\\\\\\\\n",
    "P(D) = (D^{2} - D + 2) &\\rightarrow& P(\\alpha) = \\alpha^{2}-\\alpha+2\n",
    "\\end{eqnarray*}\n",
    "\n",
    "\\begin{eqnarray*}\n",
    "(D^{2} - D + 2)\\tilde{y_{p}} &=& 10e^{(-1+i)x} \\\\\\\\\n",
    "\\Longrightarrow \\tilde{y_{p}} = \\frac{10e^{(-1+i)x}}{(-1+i)^{2}-(-1+i)+2} &=& \\frac{10e^{(-1+i)x}}{3-3i} = \\frac{5}{3}(1+i)e^{(-1+i)x}.\n",
    "\\end{eqnarray*}\n",
    "\n",
    "So the particular solution is:\n",
    "\\begin{eqnarray*}\n",
    "y_{p} = \\mathfrak{Im}(\\tilde{y_{p}}) = \\frac{5}{3}e^{-x}(\\sin{}(x)+\\cos{}(x)) = \\frac{5}{3}e^{-x}\\sqrt{2}(\\cos{}(x-\\frac{\\pi}{4}))\n",
    "\\end{eqnarray*}\n",
    "\n",
    "````\n",
    "\n",
    "````{prf:theorem}\n",
    ":label: my-theorem_erf2\n",
    "Exponential-shift theorem\n",
    "\n",
    "\\begin{eqnarray*}\n",
    "P(D)e^{ax}u(x) = e^{ax}P(D+a)u(x)\n",
    "\\end{eqnarray*}\n",
    "````\n",
    "\n",
    "````{prf:proof}\n",
    "Consider\n",
    "\\begin{eqnarray*}\n",
    "P(D)e^{ax}u(x) &=& (D^{2}+AD+B)e^{ax}u(x) \\\\\\\\\n",
    "&=& D^{2}(e^{ax}u)+AD(e^{ax}u)+B(e^{ax}u) \\\\\\\\\n",
    "&=& D(D(e^{ax}u))+AD(e^{ax}u)+B(e^{ax}u) \\\\\\\\\n",
    "&=& D(ae^{ax}u+e^{ax}Du) + A(ae^{ax}u+e^{ax}Du) + B(e^{ax}u) \\\\\\\\\n",
    "&=& e^{ax}(a^{2}u+aDu+aDu+D^{2}u+aAu+ADu+Bu) \\\\\\\\\n",
    "&=& e^{ax}(D^{2}u+2aDu+a^{2}u+A(Du+au)+Bu) \\\\\\\\\n",
    "&=& e^{ax}((D+a)^{2}u+A(D+a)u+Bu) \\\\\\\\\n",
    "&=& e^{ax}P(D+a)u(x)\n",
    "\\end{eqnarray*}\n",
    "\n",
    "````\n",
    "\n",
    "````{prf:theorem}\n",
    ":label: my-theorem_erf3\n",
    "Resonance\n",
    "\\begin{eqnarray*}\n",
    "(D^{2}+AD+B)y = e^{ax},\n",
    "\\end{eqnarray*}\n",
    "where a is complex. \n",
    "\n",
    "1. If P(a) = 0,  a is a simple root of P(D), then the particular solution is\n",
    "\n",
    "\\begin{eqnarray*}\n",
    "y_p{ = \\frac{xe^{ax}}{P'(a)}}\n",
    "\\end{eqnarray*}\n",
    "\n",
    "2. If a is a double root, then the particular solution is\n",
    "\n",
    "\\begin{eqnarray*}\n",
    "y_p{ = \\frac{x^{2}e^{ax}}{P''(a)}}\n",
    "\\end{eqnarray*}\n",
    "\n",
    "````\n",
    "\n",
    "````{prf:proof}\n",
    "1. simple root case.\n",
    "\\begin{eqnarray*}\n",
    "P(D) &=& (D-b)(D-a) = D^{2} - (a+b) + ab, a\\neq b \\\\\\\\\n",
    "P'(D) &=& (D-a) + (D-b)) \\\\\\\\\n",
    "P'(a) &=& a-b \\\\\\\\\n",
    "P(D)\\frac{xe^{ax}}{P'(a)} &=& e^{ax}\\frac{P(D+a)x}{P'(a)} \\\\\\\\\n",
    "&=& \\frac{e^{ax}(D+a-b)(D+a-a)x}{P'(a)} = \\frac{e^{ax}(D+a-b)Dx}{P'(a)} \\\\\\\\\n",
    "&=& \\frac{e^{ax}(a-b)}{a-b} = e^{ax}\n",
    "\\end{eqnarray*}\n",
    "\n",
    "````\n",
    "\n",
    "````{prf:example}\n",
    ":label: my-example_erf3\n",
    "\\begin{eqnarray*}\n",
    "y''-3y'+2y = e^{x}\\\\\\\\\n",
    "\\Longrightarrow P(D) = D^{2}-3D+2\n",
    "\\end{eqnarray*}\n",
    "So 1 is a simple root.\n",
    "\n",
    "\\begin{eqnarray*}\n",
    "P'(D) = 2D-3\\\\\\\\\n",
    "P'(1) = -1\n",
    "\\end{eqnarray*}\n",
    "\n",
    "The particular solution is\n",
    "\\begin{eqnarray*}\n",
    "y_{p} = \\frac{xe^{x}}{-1} = -xe^{x}\n",
    "\\end{eqnarray*}\n",
    "\n",
    "````\n",
    "\n",
    "````{prf:proof}\n",
    "2. double root case.\n",
    "\\begin{eqnarray*}\n",
    "P(D) &=& (D-a)(D-a) \\\\\\\\\n",
    "P'(D) &=& (D-a) + (D-a) = 2(D-a) \\\\\\\\\n",
    "P'(a) &=& 2(a-a)=0 \\\\\\\\\n",
    "P''(D) &=& 2, P''(a) = 2\\\\\\\\\n",
    "P(D)y_{p} &=& P(D)\\frac{x^{2}e^{ax}}{P''(a)}=\\frac{e^{ax}P(D+a)x^{2}}{2} \\\\\\\\\n",
    "&=& \\frac{e^{ax}Dx^{2}}{2} = e^{ax}\\frac{2Dx}{2}=e^{ax}\n",
    "\\end{eqnarray*}\n",
    "\n",
    "````"
   ]
  }
 ],
 "metadata": {
  "jupytext": {
   "text_representation": {
    "extension": ".md",
    "format_name": "myst"
   }
  },
  "kernelspec": {
   "display_name": "Python 3",
   "language": "python",
   "name": "python3"
  },
  "source_map": [
   10
  ]
 },
 "nbformat": 4,
 "nbformat_minor": 5
}