{
 "cells": [
  {
   "cell_type": "markdown",
   "id": "2313be46",
   "metadata": {},
   "source": [
    "(week7)=\n",
    "\n",
    "# Week7 - variation of parameters\n",
    "\n",
    "## The fundamental set of solutions amd Wronskian\n",
    "Consider linear ODE:\n",
    "\\begin{eqnarray*}\n",
    "&\\text{   }& y''+p(t)y'+q(t)y=0 \\\\\\\\\n",
    "y_{1}(t) \\text{ and } &y_{2}(t)& \\text{ form a fudamental set of solutions (fss) if:} \\\\\\\\\n",
    "&1.& y_{1}, y_{2} \\text{ are solutions of the ODE.} \\\\\\\\\n",
    "&2.& \\text{every solution } y(t) \\text{ of the ODE can be written as:}\\\\\\\\\n",
    "&\\text{    }& y(t) = c_{1}y_{1}(t) + c_{2}y_{2}(t)\n",
    "\\end{eqnarray*}\n",
    "\n",
    "````{prf:theorem}\n",
    ":label: my-theorem_vp1\n",
    "Two solutions form a fss if the determinat\n",
    "\n",
    "\\begin{eqnarray*}\n",
    "W(t) = \n",
    "\\begin{vmatrix}\n",
    "     y_{1}(t) & y_{2}(t) \\\\\n",
    "     y_{1}'(t) & y_{2}'(t) \n",
    "\\end{vmatrix}\n",
    "\\neq 0\n",
    "\\end{eqnarray*}\n",
    "W(t) is called Wronskian.\n",
    "\n",
    "````\n",
    "\n",
    "````{prf:example}\n",
    ":label: my-example_vp1\n",
    "Consider the ODE:\n",
    "\\begin{eqnarray*}\n",
    "y''+y=0\n",
    "\\end{eqnarray*}\n",
    "Show that\n",
    "\\begin{eqnarray*}\n",
    "y_{1}(t)=\\sin{}(t), y_{2}(t)=\\cos{}(t)\n",
    "\\end{eqnarray*}\n",
    "form a fss of this ODE.\n",
    "1. they are solutions to the ODE.\n",
    "2. \n",
    "\\begin{eqnarray*}\n",
    "W(t) =\n",
    "\\begin{vmatrix}\n",
    "     \\sin{}(t) & \\cos{}(t) \\\\\n",
    "     \\cos{}(t) & -\\sin{}(t)\n",
    "\\end{vmatrix}\n",
    "= -\\sin{}^{2}(t) - \\cos{}^{2}(t) = -1\n",
    "\\neq 0\n",
    "\\end{eqnarray*}\n",
    "\n",
    "````\n",
    "\n",
    "## Variation of parameters\n",
    "Consider the ODE:\n",
    "\\begin{eqnarray*}\n",
    "1y''+B(t)y'+C(t)y=f(t).\n",
    "\\end{eqnarray*}\n",
    "\n",
    "Suppose we have two homogeneous solutions:\n",
    "\\begin{eqnarray*}\n",
    "y_{1}(t), y_{2}(t)\n",
    "\\end{eqnarray*}\n",
    "\n",
    "The idea is to construct the particular solution as the form of\n",
    "\\begin{eqnarray*}\n",
    "y_{p}(t)=c_{1}(t)y_{1}(t) + c_{2}(t)y_{2}(t), \\\\\\\\\n",
    "c_{1}(t), c_{2}(t) \\text{ are called the varying parameters.}\n",
    "\\end{eqnarray*}\n",
    "\n",
    "if\n",
    "\\begin{eqnarray*}\n",
    "c_{1}'(t)y_{1}(t) &+& c_{2}'(t)y_{2}(t) = 0 \\\\\\\\\n",
    "c_{1}'(t)y_{1}'(t) &+& c_{2}'(t)y_{2}'(t) = f(t) \\\\\\\\\n",
    "\\Longrightarrow \n",
    "W(t) &=&\n",
    "\\begin{vmatrix}\n",
    "     y_{1}(t) & y_{2}(t) \\\\\n",
    "     y_{1}'(t) & y_{2}'(t)\n",
    "\\end{vmatrix}\n",
    "\\neq 0 \\\\\\\\\n",
    "&\\Longrightarrow& y_{1}(t), y_{2}(t) \\text{ form a fss}\n",
    "\\end{eqnarray*}\n",
    "\n",
    "then\n",
    "\\begin{eqnarray*}\n",
    "y_{p}(t) &=& y_{1}\\int{\\frac{W_{1}}{W}dt} +  y_{2}\\int{\\frac{W_{2}}{W}dt} \\\\\\\\\n",
    "W_{1} &=& \n",
    "\\begin{vmatrix}\n",
    "     0 & y_{2}(t) \\\\\n",
    "     f(t) & y_{2}'(t)\n",
    "\\end{vmatrix} \\\\\\\\\n",
    "W_{2} &=&\n",
    "\\begin{vmatrix}\n",
    "     y_{1}(t) & 0 \\\\\n",
    "     y_{1}'(t) & f(t)\n",
    "\\end{vmatrix} \\\\\\\\\n",
    "\\end{eqnarray*}\n",
    "\n",
    "So the particular solution is:\n",
    "\\begin{eqnarray*}\n",
    "y_{p}(t) = y_{1}(t)\\int{\\frac{-y_{2}(t)f(t)}{W}dt} +  y_{2}(t)\\int{\\frac{y_{1}(t)f(t)}{W}dt}\n",
    "\\end{eqnarray*}\n",
    "\n",
    "````{prf:example}\n",
    ":label: my-example_vp2\n",
    "\\begin{eqnarray*}\n",
    "y_{1}(t) = e^{s_{1}t}, y_{2}(t) = e^{s_{2}t}\n",
    "\\end{eqnarray*}\n",
    "\\begin{eqnarray*}\n",
    "W(t) = \n",
    "\\begin{vmatrix}\n",
    "     y_{1} & y_{2} \\\\\n",
    "     y_{1}' & y_{2}'\n",
    "\\end{vmatrix}\n",
    "= \n",
    "\\begin{vmatrix}\n",
    "     e^{s_{1}t} & e^{s_{2}t} \\\\\n",
    "     s_{1}e^{s_{1}t} & s_{2}e^{s_{2}t}\n",
    "\\end{vmatrix}\n",
    "=\n",
    "(s_{2}-s_{1})(e^{s_{1}t}e^{s_{2}t})\n",
    "\\end{eqnarray*}\n",
    "\n",
    "\\begin{eqnarray*}\n",
    "y_{p}(t) &=& e^{s_{1}t}\\int{\\frac{-e^{s_{2}T}f(T)}{(s_{2}-s_{1})e^{s_{1}T}e^{s_{2}T}}dT} + e^{s_{2}t}\\int{\\frac{e^{s_{1}T}f(T)}{(s_{2}-s_{1})e^{s_{1}T}e^{s_{2}T}}dT}\\\\\\\\\n",
    "&=& \\frac{-1}{s_{2}-s_{1}}\\int{e^{s_{1}(t-T)f(T)dT}} + \\frac{1}{s_{2}-s_{1}}\\int{e^{s_{2}(t-T)f(T)dT}}\\\\\\\\\n",
    "&=& \\int{g(t-T)f(T)dT}\\\\\\\\\n",
    "g(t) &=& \\frac{e^{s_{1}t}-e^{s_{2}t}}{s_{1}-s_{2}}, \\text{ growth factor}\n",
    "\\end{eqnarray*}\n",
    "\n",
    "\n",
    "````\n",
    "\n",
    "\n",
    "````{prf:example}\n",
    ":label: my-example_vp3\n",
    "\\begin{eqnarray*}\n",
    "y''=2y'+y=e^{x}\\ln{x}\n",
    "\\end{eqnarray*}\n",
    "\n",
    "1. \n",
    "\\begin{eqnarray*}\n",
    "r^2-2r+1 = 0 &\\rightarrow& (r-1)^{2} = 0 \\rightarrow y_{h}(x) = c_{1}e^{x} + c_{2}xe^{x} \\\\\\\\\n",
    "\\text{ take } y_{1}(x) &=& e^{x}, y_{2}(x) = xe^{x}\n",
    "\\end{eqnarray*}\n",
    "\n",
    "2. check\n",
    "\\begin{eqnarray*}\n",
    "y_{1}(x) \\text{ and } y_{2}(x) \\text{ form a fss}\n",
    "\\end{eqnarray*}\n",
    "\n",
    "\\begin{eqnarray*}\n",
    "W(x) &=& \n",
    "\\begin{vmatrix}\n",
    "     e^{x} & xe^{x} \\\\\n",
    "     e^{x} & e^{x}+xe^{x}\n",
    "\\end{vmatrix}\n",
    "= e^{2x}+xe^{2x}-xe^{2x} = e^{2x} \\neq 0 \\\\\\\\\n",
    "W_{1}(x) &=& \n",
    "\\begin{vmatrix}\n",
    "     0 & xe^{x} \\\\\n",
    "     e^{x}\\ln{x} & e^{x}+xe^{x}\n",
    "\\end{vmatrix}\n",
    "= -xe^{2x}\\ln{x} \\\\\\\\\n",
    "W_{2}(x) &=& \n",
    "\\begin{vmatrix}\n",
    "     e^{x} & 0 \\\\\n",
    "     e^{x} & e^{x}\\ln{x}\n",
    "\\end{vmatrix}\n",
    "= e^{2x}\\ln{x}\n",
    "\\end{eqnarray*}\n",
    "\n",
    "3. calculate the particular solution\n",
    "\\begin{eqnarray*}\n",
    "y_{p} &=& y_{1}\\int{\\frac{W_{1}}{W}dx} + y_{2}\\int{\\frac{W_{2}}{W}dx} \\\\\\\\\n",
    "&=& e^{x}\\int{\\frac{-xe^{2x}\\ln{x}}{e^{2x}}dx} + xe^{x}\\int{\\frac{e^{2x}\\ln{x}}{e^{2x}}dx} \\\\\\\\\n",
    "&=& -e^{x}\\int{x\\ln{x}dx} + xe^{x}\\int{\\ln{x}dx}\\\\\\\\\n",
    "&=& -e^{x}(\\frac{1}{2}x^{2}\\ln{x}-\\frac{1}{2}\\int{xdx}) + xe^{x}(x\\ln{x}-\\int{xd\\ln{x}})\\\\\\\\\n",
    "&=& -e^{x}(\\frac{1}{2}x^{2}\\ln{x}-\\frac{1}{4}x^{2}) + xe^{2}(x\\ln{x}-x)\n",
    "\\end{eqnarray*}\n",
    "\n",
    "4. caclulate the general solution\n",
    "\\begin{eqnarray*}\n",
    "y(x) = y_{h}(x) + y_{p}(x)\n",
    "\\end{eqnarray*}\n",
    "\n",
    "````"
   ]
  }
 ],
 "metadata": {
  "jupytext": {
   "text_representation": {
    "extension": ".md",
    "format_name": "myst"
   }
  },
  "kernelspec": {
   "display_name": "Python 3",
   "language": "python",
   "name": "python3"
  },
  "source_map": [
   10
  ]
 },
 "nbformat": 4,
 "nbformat_minor": 5
}